[minor] Lemmas for word arithmetic.
Borrowed most of the structure and proofs from ssreflect.
The scope key for words is now "w" instead of "word".
Also started to chase some admits in refinement proof for memory safety.

lib/utils.v
@@ -1912,3 +1912,117 @@ Fixpoint sequence A n (v : Vector.t (option A) n) : option (Vector.t A n) :=
   end.
 
 End vectors.
+
+(* Borrowed from ssr *)
+Module Option.
+
+Definition apply aT rT (f : aT -> rT) x u :=
+  match u with Some y => f y | _ => x end.
+
+Definition default T := apply (fun x : T => x).
+
+Definition bind aT rT (f : aT -> option rT) := apply f None.
+
+Definition map aT rT (f : aT -> rT) := bind (fun x => Some (f x)).
+
+End Option.
+
+Notation oapp := Option.apply.
+Notation odflt := Option.default.
+Notation obind := Option.bind.
+Notation omap := Option.map.
+Notation some := (@Some _) (only parsing).
+
+Section Injections.
+
+(* rT must come first so we can use @ to mitigate the Coq 1st order   *)
+(* unification bug (e..g., Coq can't infer rT from a "cancel" lemma). *)
+Variables (rT aT : Type) (f : aT -> rT).
+
+Definition injective := forall x1 x2, f x1 = f x2 -> x1 = x2.
+
+Definition pcancel g := forall x, g (f x) = Some x.
+
+Definition ocancel (g : aT -> option rT) h := forall x, oapp h x (g x) = x.
+
+Definition cancel g := forall x, g (f x) = x.
+
+Lemma can_pcan g : cancel g -> pcancel (fun y => Some (g y)).
+Proof. now intros fK x; rewrite fK. Qed.
+
+Lemma pcan_inj g : pcancel g -> injective.
+Proof.
+intros fK x y eq_f.
+apply (f_equal g) in eq_f.
+rewrite !fK in eq_f.
+now injection eq_f as ->.
+Qed.
+
+Lemma can_inj g : cancel g -> injective.
+Proof.
+intros can_g; apply can_pcan in can_g.
+now revert can_g; apply pcan_inj.
+Qed.
+
+End Injections.
+
+Lemma Some_inj {T} : injective (@Some T).
+Proof. now intros x y H; injection H. Qed.
+
+(* Notations for argument transpose *)
+Notation "f ^~ y" := (fun x => f x y)
+  (at level 10, y at level 8, no associativity, format "f ^~  y") : fun_scope.
+Notation "@^~ x" := (fun f => f x)
+  (at level 10, x at level 8, no associativity, format "@^~  x") : fun_scope.
+
+Section OperationProperties.
+
+Open Scope fun_scope.
+
+Variables S T R : Type.
+
+Section SopTisR.
+Implicit Type op :  S -> T -> R.
+Definition left_inverse e inv op := forall x, op (inv x) x = e.
+Definition right_inverse e inv op := forall x, op x (inv x) = e.
+Definition left_injective op := forall x, injective (op^~ x).
+Definition right_injective op := forall y, injective (op y).
+End SopTisR.
+
+Section SopTisS.
+Implicit Type op :  S -> T -> S.
+Definition right_id e op := forall x, op x e = x.
+Definition left_zero z op := forall x, op z x = z.
+Definition right_commutative op := forall x y z, op (op x y) z = op (op x z) y.
+Definition left_distributive op add :=
+  forall x y z, op (add x y) z = add (op x z) (op y z).
+Definition right_loop inv op := forall y, cancel (op^~ y) (op^~ (inv y)).
+Definition rev_right_loop inv op := forall y, cancel (op^~ (inv y)) (op^~ y).
+End SopTisS.
+
+Section SopTisT.
+Implicit Type op :  S -> T -> T.
+Definition left_id e op := forall x, op e x = x.
+Definition right_zero z op := forall x, op x z = z.
+Definition left_commutative op := forall x y z, op x (op y z) = op y (op x z).
+Definition right_distributive op add :=
+  forall x y z, op x (add y z) = add (op x y) (op x z).
+Definition left_loop inv op := forall x, cancel (op x) (op (inv x)).
+Definition rev_left_loop inv op := forall x, cancel (op (inv x)) (op x).
+End SopTisT.
+
+Section SopSisT.
+Implicit Type op :  S -> S -> T.
+Definition self_inverse e op := forall x, op x x = e.
+Definition commutative op := forall x y, op x y = op y x.
+End SopSisT.
+
+Section SopSisS.
+Implicit Type op :  S -> S -> S.
+Definition idempotent op := forall x, op x x = x.
+Definition associative op := forall x y z, op x (op y z) = op (op x y) z.
+Definition interchange op1 op2 :=
+  forall x y z t, op1 (op2 x y) (op2 z t) = op2 (op1 x z) (op1 y t).
+End SopSisS.
+
+End OperationProperties.
