concrete/common.v
@@ -4,6 +4,8 @@ Require Import ZArith.
 Require Import Bool.
 Require Import Coq.Classes.SetoidDec.
 
+Require Import utils.
+
 Import ListNotations.
 
 Set Implicit Arguments.
@@ -108,11 +110,14 @@ Class machine_ops (t : machine_types) := {
   imm_to_word : imm t -> word t;
 
   (* CH: I think it would be nicer to have Z_to_imm be partial *)
+  zero_word : word t;
+
+  max_word : word t;
   Z_to_word : Z -> word t;
   word_to_Z : word t -> Z;
 
   add_word : word t -> word t -> word t;
-  sub_word : word t -> word t -> word t;
+  opp_word : word t -> word t;
   eq_word :> EqDec (eq_setoid (word t));
 
   eq_reg :> EqDec (eq_setoid (word t));
@@ -121,19 +126,109 @@ Class machine_ops (t : machine_types) := {
 
 }.
 
+Notation "x + y" := (add_word x y) : word_scope.
+Notation "- x" := (opp_word x) : word_scope.
+Notation "x - y" := (add_word x (opp_word y)) : word_scope.
+Notation "0" := zero_word : word_scope.
+Notation "+%w" := add_word.
+Notation "-%w" := opp_word.
+
+Delimit Scope word_scope with w.
+
 (* CH: At some point should prove or at least test that the concrete
    instantiation satisfies these *)
 Class machine_ops_spec t (ops : machine_ops t) := {
 
   decodeK : forall i, decode_instr (encode_instr i) = Some i;
 
+  max_word_bound : (15 < word_to_Z max_word)%Z;
+
   word_to_ZK : forall w, Z_to_word (word_to_Z w) = w;
 
   Z_to_wordK : forall z,
-                 (0 <= z <= 255)%Z ->
-                 word_to_Z (Z_to_word z) = z
+                 (0 <= z <= word_to_Z max_word)%Z ->
+                 word_to_Z (Z_to_word z) = z;
+
+  zerowP : word_to_Z 0%w = 0%Z;
+
+  addwP : forall w1 w2, word_to_Z (w1 + w2)%w = (word_to_Z w1 + word_to_Z w2)%Z;
+
+  oppwP : forall w, word_to_Z (- w)%w = (- word_to_Z w)%Z
 
 }.
+
+Section WordArith.
+
+Local Open Scope word_scope.
+
+Context {t : machine_types}
+        {op : machine_ops t}
+        {ops : machine_ops_spec op}.
+
+Lemma word_to_Z_inj : injective word_to_Z.
+Proof. exact (can_inj word_to_ZK). Qed.
+
+Ltac toZ := apply word_to_Z_inj; repeat rewrite ?zerowP, ?addwP, ?oppwP.
+
+Lemma addwA : associative +%w.
+Proof.
+now intros w1 w2 w3; toZ; rewrite Z.add_assoc.
+Qed.
+
+Lemma addwC : commutative +%w.
+Proof. 
+now intros w1 w2; toZ; rewrite Z.add_comm.
+Qed.
+
+Lemma add0w : left_id 0 +%w.
+Proof.
+now intros w; toZ; rewrite Z.add_0_l.
+Qed.
+
+Lemma addNw : left_inverse 0 -%w +%w.
+Proof.
+now intros w; toZ; rewrite Z.add_opp_diag_l. (* What a name! *)
+Qed.
+
+Lemma addw0 : right_id 0 +%w.
+Proof. now intros x; rewrite addwC, add0w. Qed.
+
+Lemma addwN : right_inverse 0 -%w +%w.
+Proof. now intros x; rewrite addwC, addNw. Qed.
+Definition subww := addwN.
+
+Lemma addKw : left_loop -%w +%w.
+Proof.
+now intros x y; rewrite addwA, addNw, add0w.
+Qed.
+
+Lemma addNKw : rev_left_loop -%w +%w.
+Proof. 
+now intros x y; rewrite addwA, addwN, add0w.
+Qed.
+
+Lemma addwK : right_loop -%w +%w.
+Proof. 
+now intros x y; rewrite <-addwA, addwN, addw0.
+Qed.
+
+Lemma addwNK : rev_right_loop -%w +%w.
+Proof.
+now intros x y; rewrite <-addwA, addNw, addw0.
+Qed.
+
+Definition subwK := addwNK.
+
+Lemma addwI : right_injective +%w.
+Proof. intros x; exact (can_inj (addKw x)). Qed.
+
+Lemma addIw : left_injective +%w.
+Proof. intros y; exact (can_inj (addwK y)). Qed.
+
+(* If more lemmas are needed, please copy the statements and proofs
+from ssralg.v in ssreflect to keep the nice structure. *)
+
+End WordArith.
 
 Section Coding.
 
@@ -191,19 +286,17 @@ Definition word_to_op (w : word t) : option opcode :=
 Definition op_to_word (o : opcode) : word t :=
   Z_to_word (op_to_Z o).
 
-Lemma op_to_wordK (o : opcode) : word_to_op (op_to_word o) = Some o.
+Lemma op_to_wordK : pcancel op_to_word word_to_op.
 Proof.
-  unfold word_to_op, op_to_word.
-  rewrite Z_to_wordK; destruct o; try reflexivity; simpl; try omega;
-  destruct b; try reflexivity; omega.
+  unfold pcancel, word_to_op, op_to_word; intros o.
+  assert (H := max_word_bound).
+  rewrite Z_to_wordK; destruct o; try reflexivity; simpl; try omega;   destruct b; try reflexivity; omega.
 Qed.
 
-Lemma word_to_opK o o' :
-  word_to_op o = Some o' ->
-  op_to_word o' = o.
+Lemma word_to_opK : ocancel word_to_op op_to_word.
 Proof.
-  unfold word_to_op, op_to_word.
-  intros H.
+  unfold ocancel, oapp, word_to_op, op_to_word.
+  intros o; destruct (Z_to_op (word_to_Z o)) as [o'|] eqn:H; try reflexivity.
   remember (word_to_Z o) as w.
   unfold Z_to_op in H.
   repeat match goal with
@@ -218,22 +311,13 @@ Proof.
   apply word_to_ZK.
 Qed.
 
-Lemma op_to_word_inj (o1 o2 : opcode) : op_to_word o1 = op_to_word o2 -> o1 = o2.
-Proof.
-  intros H.
-  cut (Some o1 = Some o2); try congruence.
-  do 2 rewrite <- op_to_wordK. congruence.
-Qed.
+Lemma op_to_word_inj : injective op_to_word.
+Proof. now apply (pcan_inj op_to_wordK). Qed.
 
 Definition op_to_imm (o : opcode) : imm t :=
   Z_to_imm (op_to_Z o).
 
 End Coding.
-
-Notation "x + y" := (add_word x y) : word_scope.
-Notation "x - y" := (sub_word x y) : word_scope.
-
-Delimit Scope word_scope with word.
 
 Record atom V T := Atom { val : V; tag : T }.
 
